my changes

code/salsa-family/Hacl.Impl.Chacha20.fst
@@ -99,14 +99,6 @@ let rounds st =
   iter 10 Spec.double_round double_round st
 
 
-val copy_state: o:state -> i:state -> Stack unit 
-		(requires (fun h -> live h o /\ live h i))
-		(ensures (fun h0 _ h1 -> preserves_live h0 h1 /\ modifies1 o h0 h1 /\
-			       as_lseq o h1 == as_lseq i h0))
-let copy_state o i = 
-  admit();
-  blit i 0 o 0 16
-
 [@ "c_inline"]
 private
 val chacha20_core:
@@ -122,7 +114,7 @@ val chacha20_core:
 [@ "c_inline"]
 let chacha20_core k st ctr =
   st.(12) <- u32 ctr;
-  copy_state k st;
+  copy st k;
   rounds k;
   map2 (fun x y -> x +. y) k st
 
@@ -131,28 +123,26 @@ val setup:
   st:state ->
   k:lbuffer uint8 32 ->
   n:lbuffer uint8 12 ->
-  c:size_t ->
   Stack unit
     (requires (fun h -> live h st /\ live h k /\ live h n
                     /\ disjoint k st /\ disjoint n st))
     (ensures (fun h0 _ h1 -> preserves_live h0 h1 /\ modifies1 st h0 h1
                        /\ as_lseq st h1 == 
-			 Spec.setup (as_lseq k h0) (as_lseq n h0) c (as_lseq st h0)))
+			 Spec.setup (as_lseq k h0) (as_lseq n h0) (as_lseq st h0)))
 
 #reset-options "--z3rlimit 50 --max_fuel 0"
 [@ "c_inline"]
-let setup st k n c =
+let setup st k n =
   st.(0) <- u32 Spec.c0;
   st.(1) <- u32 Spec.c1;
   st.(2) <- u32 Spec.c2;
   st.(3) <- u32 Spec.c3;
   let st_k = sub st 4 8 in
   uint32s_from_bytes_le #8 st_k k;
-  st.(12) <- u32 c;
   let st_n = sub st 13 3 in
   uint32s_from_bytes_le #3 st_n n 
 
-
+(*
 [@ "c_inline"]
 val chacha20_block:
   stream_block:lbuffer uint8 64 ->
@@ -162,7 +152,10 @@ val chacha20_block:
     (requires (fun h -> live h stream_block /\ 
 		     live h st /\ 
 		     disjoint stream_block st))
-    (ensures  (fun h0 _ h1 -> preserves_live h0 h1 /\ modifies2 st stream_block h0 h1))
+    (ensures  (fun h0 _ h1 -> preserves_live h0 h1 /\ modifies2 st stream_block h0 h1 /\
+			   as_lseq st h1 == 
+			   Spec.chacha20_block stream_block st ctrsetup (as_lseq k h0) (as_lseq n h0) c (as_lseq st h0)))
+			   ))
 
 #reset-options "--z3rlimit 100"
 [@ "c_inline"]
@@ -178,120 +171,29 @@ let chacha20_block stream_block st ctr =
   alloc 16 (u32 0) bufs spec impl
     
 
-
-(*
 [@ "c_inline"]
 val init:
   st:state ->
   k:lbuffer uint8 32 ->
   n:lbuffer uint8 12 ->
-  Stack log_t
-    (requires (fun h -> live h k /\ live h n /\ live h st /\ disjoint st k /\ disjoint st n /\ disjoint k n))
-    (ensures  (fun h0 log h1 -> preserves_live h0 h1 /\ modifies1 st h0 h1))
-      // /\ invariant log h1 st
-      // /\ (match Ghost.reveal log with MkLog k' n' -> k' == reveal_sbytes (as_seq h0 k)
-      //      /\ n' == reveal_sbytes (as_seq h0 n))))
-
+  Stack unit
+    (requires (fun h -> live h k /\ live h n /\ live h st /\ disjoint k st /\ disjoint n st))
+    (ensures  (fun h0 _ h1 -> preserves_live h0 h1 /\ modifies1 st h0 h1))
 [@ "c_inline"]
 let init st k n =
-  setup st k n 0;
-  let h = ST.get() in
-  Ghost.elift2 (fun (k:lbuffer uint8 32) (n:lbuffer uint8 12) -> MkLog (as_lseq k h) (as_lseq n h)) (Ghost.hide k) (Ghost.hide n)
-
-
-(*
-#reset-options " --max_fuel 0 --z3rlimit 100"
-
-val lemma_chacha20_counter_mode_1:
-  ho:mem -> output:uint8_p{live ho output} ->
-  hi:mem -> input:uint8_p{live hi input} ->
-  len:U32.t{U32.v len = length output /\ U32.v len = length input /\ U32.v len < 64 /\ U32.v len > 0} ->
-  k:Spec.key -> n:Spec.nonce -> ctr:UInt32.t{UInt32.v ctr + (length input / 64) < pow2 32} -> Lemma
-    (Spec.CTR.counter_mode chacha20_ctx chacha20_cipher k n (UInt32.v ctr) (reveal_sbytes (as_seq hi input))
-     == Spec.CTR.xor #(UInt32.v len) (reveal_sbytes (as_seq hi input)) (Seq.slice (Spec.chacha20_block k n (UInt32.v ctr)) 0 (U32.v len)))
-#reset-options "--max_fuel 0 --z3rlimit 100"
-let lemma_chacha20_counter_mode_1 ho output hi input len k n ctr =
-  Math.Lemmas.lemma_div_mod (UInt32.v len) 64;
-  Math.Lemmas.modulo_lemma (UInt32.v len) 64;
-  assert(UInt32.v len / (Spec.CTR.(chacha20_ctx.blocklen * chacha20_ctx.incr)) = 0);
-  let open Spec.CTR in
-  assert((xor #(UInt32.v len) (reveal_sbytes (as_seq hi input)) (Seq.slice (Spec.chacha20_block k n (UInt32.v ctr)) 0 (UInt32.v len))) == seq_map2 (fun x y -> FStar.UInt8.(x ^^ y)) (reveal_sbytes (as_seq hi input)) (Seq.slice (Spec.chacha20_block k n (UInt32.v ctr)) 0 (UInt32.v len)));
-  let ctx = chacha20_ctx in
-  let len:nat = UInt32.v len in
-  let counter = UInt32.v ctr in
-  let blocks_len = (ctx.incr * ctx.blocklen) * (len / (ctx.blocklen * ctx.incr)) in
-  let part_len   = len % (ctx.blocklen * ctx.incr) in
-    (* TODO: move to a single lemma for clarify *)
-    Math.Lemmas.lemma_div_mod len (ctx.blocklen * ctx.incr);
-    Math.Lemmas.multiple_modulo_lemma (len / (ctx.blocklen * ctx.incr)) (ctx.blocklen * ctx.incr);
-    Math.Lemmas.lemma_div_le (blocks_len) len ctx.blocklen;
-    (* End TODO *)
-  let blocks, last_block = Seq.split (as_seq hi input) blocks_len in
-  let cipher_blocks = counter_mode_blocks ctx chacha20_cipher k n counter (reveal_sbytes blocks) in
-  Seq.lemma_eq_intro cipher_blocks Seq.createEmpty;
-  assert(ctx.incr * (Seq.length (as_seq hi input) / ctx.blocklen) = 0);
-  Seq.lemma_eq_intro (Seq.append Seq.createEmpty (xor #len (reveal_sbytes (as_seq hi input)) (Seq.slice (Spec.chacha20_block k n (UInt32.v ctr)) 0 len))) (xor #len (reveal_sbytes (as_seq hi input)) (Seq.slice (Spec.chacha20_block k n (UInt32.v ctr)) 0 len));
-  Seq.lemma_eq_intro (Spec.CTR.counter_mode chacha20_ctx chacha20_cipher k n (UInt32.v ctr) (reveal_sbytes (as_seq hi input)))
-                     (Spec.CTR.xor #(len) (reveal_sbytes (as_seq hi input)) (Seq.slice (Spec.chacha20_block k n (UInt32.v ctr)) 0 (len)))
-
-
-#reset-options " --max_fuel 0 --z3rlimit 100"
-
-val lemma_chacha20_counter_mode_2:
-  ho:mem -> output:uint8_p{live ho output} ->
-  hi:mem -> input:uint8_p{live hi input} ->
-  len:U32.t{U32.v len = length output /\ U32.v len = length input /\ U32.v len >= 64
-    /\ UInt32.v len % 64 = 0} ->
-  k:Spec.key -> n:Spec.nonce -> ctr:UInt32.t{UInt32.v ctr + (length input / 64) < pow2 32} -> Lemma
-    (Spec.CTR.counter_mode_blocks chacha20_ctx chacha20_cipher k n (UInt32.v ctr)
-                                  (reveal_sbytes (as_seq hi input))
-    == (let prefix, block = Seq.split (as_seq hi input) (UInt32.v len - 64) in    
-      Math.Lemmas.lemma_mod_plus (Seq.length prefix) 1 (64);
-      Math.Lemmas.lemma_div_le (Seq.length prefix) (UInt32.v len) 64;
-      Spec.CTR.Lemmas.lemma_div (UInt32.v len) (64);
-    let cipher        = Spec.CTR.counter_mode_blocks chacha20_ctx chacha20_cipher k n (UInt32.v ctr) (reveal_sbytes prefix) in
-    let mask          = chacha20_cipher k n (UInt32.v ctr + (UInt32.v len / 64 - 1) ) in
-    let eb            = Spec.CTR.xor (reveal_sbytes block) mask in
-    Seq.append cipher eb))
-#reset-options "--initial_fuel 1 --max_fuel 1 --z3rlimit 100"
-let lemma_chacha20_counter_mode_2 ho output hi input len k n ctr = ()
-
-
-#reset-options " --max_fuel 0 --z3rlimit 100"
-
-val lemma_chacha20_counter_mode_0:
-  ho:mem -> output:uint8_p{live ho output} ->
-  hi:mem -> input:uint8_p{live hi input} ->
-  len:U32.t{U32.v len = length output /\ U32.v len = length input /\ U32.v len = 0} ->
-  k:Spec.key -> n:Spec.nonce -> ctr:UInt32.t{UInt32.v ctr + (length input / 64) < pow2 32} -> Lemma
-    (Spec.CTR.counter_mode_blocks chacha20_ctx chacha20_cipher k n (UInt32.v ctr)
-                                  (reveal_sbytes (as_seq hi input))
-     == Seq.createEmpty)
-#reset-options "--initial_fuel 1 --max_fuel 1 --z3rlimit 100"
-let lemma_chacha20_counter_mode_0 ho output hi input len k n ctr =
-  Seq.lemma_eq_intro (as_seq ho output) Seq.createEmpty
-*)
-
+  setup st k n 0
+  
 #reset-options " --max_fuel 0 --z3rlimit 400"
 
 val update_last:
   len:size_t{0 < len /\ len < 64} ->
   output:lbuffer uint8 len ->
   plain:lbuffer uint8 len ->
-  log:log_t ->
   st:state ->
   ctr:size_t{ctr + (len / 64) <= max_size_t} ->
-  Stack log_t
+  Stack unit
     (requires (fun h -> live h output /\ live h plain /\ disjoint output plain /\ disjoint st output /\ disjoint st plain)) //invariant log h st))
-    (ensures (fun h0 updated_log h1 -> preserves_live h0 h1 /\ modifies2 output st h0 h1))
-      // live h1 output /\ live h0 plain /\ invariant updated_log h1 st
-      // /\ (let o = reveal_sbytes (as_seq h1 output) in
-      //    let plain = reveal_sbytes (as_seq h0 plain) in
-      //    match Ghost.reveal log with | MkLog k n ->
-      //    o == (let mask = chacha20_cipher k n (UInt32.v ctr+(UInt32.v len / 64)) in
-      //          let mask = Seq.slice mask 0 (UInt32.v len) in
-      //          Spec.CTR.xor #(UInt32.v len) plain mask))))
-
+    (ensures (fun h0 _ h1 -> preserves_live h0 h1 /\ modifies2 output st h0 h1))
 let update_last len output plain log st ctr =
   (**) let h0 = ST.get() in
   push_frame();
