specs/Spec.Chacha20.fst
@@ -65,32 +65,29 @@ let c1 = 0x3320646e
 let c2 = 0x79622d32
 let c3 = 0x6b206574
 
-let setup (k:key) (n:nonce) (c:counter) (st:state) : Tot state =
+let setup (k:key) (n:nonce) (st:state) : Tot state =
   let st = st.[0] <- u32 c0 in
   let st = st.[1] <- u32 c1 in
   let st = st.[2] <- u32 c2 in
   let st = st.[3] <- u32 c3 in
   let st = update_sub st 4 8 (uints_from_bytes_le k) in
-  let st = st.[12] <- u32 c in
   let st = update_sub st 13 3 (uints_from_bytes_le n) in
   st
 
-let chacha20_block (k:key) (n:nonce) (c:counter): Tot block =
+let chacha20_init (k:key) (n:nonce) : Tot state = 
   let st = create 16 (u32 0) in
-  let st  = setup k n c st in
+  let st  = setup k n st in
+  st
+
+let chacha20_set_counter (st:state) (c:counter) : Tot state =
+  st.[12] <- (u32 c)
+  
+let chacha20_key_block (st:state) : Tot block =
   let st' = chacha20_core st in
   uints_to_bytes_le st'
 
-let chacha20_ctx: Spec.CTR.block_cipher_ctx =
-  let open Spec.CTR in
-  {
-    keylen = keylen;
-    blocklen = blocklen;
-    noncelen = noncelen;
-    countermax = 1
-  }
-
-let chacha20_cipher: Spec.CTR.block_cipher chacha20_ctx = chacha20_block
+let chacha20_cipher = 
+  Spec.CTR.Cipher state keylen noncelen max_size_t blocklen chacha20_init chacha20_set_counter chacha20_key_block
 
 let chacha20_encrypt_bytes key nonce counter m =
-    Spec.CTR.counter_mode chacha20_ctx chacha20_cipher key nonce counter m
+    Spec.CTR.counter_mode chacha20_cipher key nonce counter m
